\documentclass{article}

	% Packages
	\usepackage[utf8]{inputenc} % UTF-8 encoding
	\usepackage[T1]{fontenc} % Font encoding
	\usepackage{lipsum} % For generating dummy text, can be removed

	\begin{document}

	 Today we will study integrals

$$\int \arctan{x}dx = \frac{1}{1+x^2}\arctan{x} + C$$

$$\frac{d}{dx}(4x^2+3x) = 8x+3$$ \documentclass[12pt]{article}
\usepackage{amsmath}
\usepackage{amsfonts}
\usepackage{amssymb}

\begin{document}

\noindent **Problem 7.1.6**

$$\int x^2 e^{3x}dx = ?$$

We can solve this integral by using integration by parts. Let \(u = x^2\) and \(dv = e^{3x}dx\). Then \(du = 2x dx\) and \(v = \frac{1}{3}e^{3x}\). Substituting into the formula for integration by parts, we get:

$$\int x^2 e^{3x}dx = \frac{1}{3}x^2 e^{3x} - \int \frac{2}{3}xe^{3x}dx$$

Now, we can use integration by parts again to evaluate the remaining integral. Let \(u = \frac{2}{3}x\) and \(dv = e^{3x}dx\). Then \(du = \frac{2}{3}dx\) and \(v = \frac{1}{3}e^{3x}\). Substituting into the formula for integration by parts, we get:

$$\int \frac{2}{3}xe^{3x}dx = \frac{1}{3}x e^{3x} - \int \frac{2}{9}e^{3x}dx$$

Combining this result with the previous one, we get:

$$\int x^2 e^{3x}dx = \frac{1}{3}x^2 e^{3x} - \frac{1}{3}x e^{3x} + \int \frac{2}{9}e^{3x}dx$$

Now, we can evaluate the remaining integral by using the power rule of integration. We get:

$$\int x^2 e^{3x}dx = \frac{1}{3}x^2 e^{3x} - \frac{1}{3}x e^{3x} + \frac{2}{9} \cdot \frac{1}{3}e^{3x} + C$$

Simplifying, we get:

$$\int x^2 e^{3x}dx = \frac{1}{3}x^2 e^{3x} - \frac{1}{3}x e^{3x} + \frac{2}{9}e^{3x} + C$$

where \(C\) is the constant of integration.

\end{document}